Problem:
Find the characteristic polynomial of the following matrix:
$\left(
  \begin{array}{ccc}
    0  & 6  & -1 \\
    -4 & -9 & -5 \\
    -7 & 1  & -2 \\
  \end{array}
  \right)$
Answer:
\begin{array}{l}

  \begin{array}{l}
    \text{Find the characteristic polynomial of the matrix }M\text{ with respect to the variable }\lambda : \\
    M=\left(
    \begin{array}{ccc}
        0  & 6  & -1 \\
        -4 & -9 & -5 \\
        -7 & 1  & -2 \\
      \end{array}
    \right)                                                                                                 \\
  \end{array}
  \\
  \hline

  \begin{array}{l}
    \text{To }\text{find }\text{the }\text{characteristic }\text{polynomial }\text{of }\text{a }\text{matrix, }\text{subtract }\text{a }\text{variable }\text{multiplied }\text{by }\text{the }\text{identity }\text{matrix }\text{and }\text{take }\text{the }\text{determinant}: \\
    | M-\lambda  \mathbb{I}|                                                                                                                                                                                                                                                       \\
  \end{array}
  \\

  \begin{array}{l}

    \begin{array}{lll}
      | M-\lambda  \mathbb{I}| & = & \left|
      \begin{array}{ccc}
        0  & 6  & -1 \\
        -4 & -9 & -5 \\
        -7 & 1  & -2 \\
      \end{array}
      -\lambda
      \begin{array}{ccc}
        1 & 0 & 0 \\
        0 & 1 & 0 \\
        0 & 0 & 1 \\
      \end{array}
      \right|                               \\
      \text{}                  & = & \left|
      \begin{array}{ccc}
        0  & 6  & -1 \\
        -4 & -9 & -5 \\
        -7 & 1  & -2 \\
      \end{array}
      -
      \begin{array}{ccc}
        \lambda & 0       & 0       \\
        0       & \lambda & 0       \\
        0       & 0       & \lambda \\
      \end{array}
      \right|                               \\
    \end{array}
    \\
    \text{= }\left|
    \begin{array}{ccc}
      -\lambda & 6           & -1          \\
      -4       & -\lambda -9 & -5          \\
      -7       & 1           & -\lambda -2 \\
    \end{array}
    \right| \\
  \end{array}
  \\

  \begin{array}{l}
    \text{Row }3 \text{has }\text{as }\text{many }\text{or }\text{more }\text{ones }\text{than }\text{the }\text{others}: \\
    \text{= }\left|
    \begin{array}{ccc}
      -\lambda & 6           & -1          \\
      -4       & -\lambda -9 & -5          \\
      -7       & 1           & -\lambda -2 \\
    \end{array}
    \right|                                                                                                               \\
  \end{array}
  \\

  \begin{array}{l}
    \text{The }\text{determinant }\text{of }\text{the }\text{matrix }\left(
    \begin{array}{ccc}
        -\lambda & 6           & -1          \\
        -4       & -\lambda -9 & -5          \\
        -7       & 1           & -\lambda -2 \\
      \end{array}
    \right) \text{is }\text{given }\text{by }(-7)\, \left|
    \begin{array}{cc}
      6           & -1 \\
      -\lambda -9 & -5 \\
    \end{array}
    \right| +(-1)\, \left|
    \begin{array}{cc}
      -\lambda & -1 \\
      -4       & -5 \\
    \end{array}
    \right| +(-\lambda -2) \left|
    \begin{array}{cc}
      -\lambda & 6           \\
      -4       & -\lambda -9 \\
    \end{array}
    \right| : \\
    \text{= }(-7)\, \left|
    \begin{array}{cc}
      6           & -1 \\
      -\lambda -9 & -5 \\
    \end{array}
    \right| +(-1)\, \left|
    \begin{array}{cc}
      -\lambda & -1 \\
      -4       & -5 \\
    \end{array}
    \right| +(-\lambda -2) \left|
    \begin{array}{cc}
      -\lambda & 6           \\
      -4       & -\lambda -9 \\
    \end{array}
    \right|   \\
  \end{array}
  \\

  \begin{array}{l}
    (-7)\, \left|
    \begin{array}{cc}
      6           & -1 \\
      -\lambda -9 & -5 \\
    \end{array}
    \right| =(-7)\, (6 (-5)-(-1)\, -\lambda -9)=-7 (-\lambda -39)=\fbox{$-7 (-\lambda -39)$}: \\
    \text{= }\fbox{$-7 (-\lambda -39)$}+(-1)\, \left|
    \begin{array}{cc}
      -\lambda & -1 \\
      -4       & -5 \\
    \end{array}
    \right| +(-\lambda -2) \left|
    \begin{array}{cc}
      -\lambda & 6           \\
      -4       & -\lambda -9 \\
    \end{array}
    \right|                                                                                   \\
  \end{array}
  \\

  \begin{array}{l}
    (-1)\, \left|
    \begin{array}{cc}
      -\lambda & -1 \\
      -4       & -5 \\
    \end{array}
    \right| =(-1)\, (5 \lambda -(-1)\, (-4))=-(5 \lambda -4)=\fbox{$4-5 \lambda $}: \\
    \text{= }-7 (-\lambda -39)+\fbox{$4-5 \lambda $}+(-\lambda -2) \left|
    \begin{array}{cc}
      -\lambda & 6           \\
      -4       & -\lambda -9 \\
    \end{array}
    \right|                                                                         \\
  \end{array}
  \\

  \begin{array}{l}
    (-\lambda -2) \left|
    \begin{array}{cc}
      -\lambda & 6           \\
      -4       & -\lambda -9 \\
    \end{array}
    \right| =(-\lambda -2) ((-\lambda ) (-\lambda -9)-6 (-4))=(-\lambda -2) \left(\lambda ^2+9 \lambda +24\right)=\fbox{$(-\lambda -2) \left(\lambda ^2+9 \lambda +24\right)$}: \\
    \text{= }-7 (-\lambda -39)+(4-5 \lambda )+\fbox{$(-\lambda -2) \left(\lambda ^2+9 \lambda +24\right)$}                                                                      \\
  \end{array}
  \\

  \begin{array}{l}
    -7 (-\lambda -39)+(4-5 \lambda )+\fbox{$(-\lambda -2) \left(\lambda ^2+9 \lambda +24\right)$}\, =\, -\lambda ^3-11 \lambda ^2-40 \lambda +229: \\
    \fbox{$
        \begin{array}{ll}
          \text{Answer:} &                                                    \\
          \text{}        & \text{= }-\lambda ^3-11 \lambda ^2-40 \lambda +229 \\
        \end{array}
    $}                                                                                                                                             \\
  \end{array}
  \\
\end{array}
